Transfer some results from combinator to de Bruijn form

src/Terms.v
@@ -1,4 +1,4 @@
-(** * Lambda calculus parametric de Bruijn terms *)
+(** * Lambda calculus with parametric de Bruijn terms *)
 
 (**
   We use the parametric de Bruijn convention of
@@ -9,71 +9,33 @@
 
 Definition Succ := S%nat.  (* an alias for later *)
 
-Require Import Coq.Program.Basics.
-Require Import Coq.Program.Equality.
-Require Import Coq.Setoids.Setoid.
-Require Import Coq.Classes.RelationClasses.
-Require Import Coq.Classes.Morphisms.
 Require Export Notations.
 
 (** ** Terms *)
 
-Inductive term {Var : Set} : Set :=
-  | TOP : term
-  | BOT : term
-  | JOIN : term -> term -> term
-  | RAND : term -> term -> term
-  | APP : term -> term -> term
-  | VAR : Var -> term
-  | LAMBDA : @term (option Var) -> term
+Inductive Term {Var : Set} : Set :=
+  | TOP : Term
+  | BOT : Term
+  | JOIN : Term -> Term -> Term
+  | RAND : Term -> Term -> Term
+  | APP : Term -> Term -> Term
+  | VAR : Var -> Term
+  | LAMBDA : @Term (option Var) -> Term
 .
-Hint Constructors term.
-Definition Term (Var : Set) := @term Var.
-Definition Closed := @term Empty_set.
+Arguments Term : default implicits.
+Hint Constructors Term.
+Definition Closed := Term Empty_set.
 
 Notation "x * y" := (APP x y) : term_scope.
 Open Scope term_scope.
 Delimit Scope term_scope with term.
-Bind Scope term_scope with term.
+Bind Scope term_scope with Term.
 
 Notation "x * y" := (APP x y) : term_scope.
 Notation "x || y" := (JOIN x y) : term_scope.
 Notation "x (+) y" := (RAND x y) : term_scope.
 
-(* adapted from https://coq.inria.fr/cocorico/UntypedLambdaTerms *)
-
-Fixpoint term_map {Var Var' : Set} (h : Var -> Var') (t : Term Var) :
-  Term Var' :=
-  match t with
-  | TOP => TOP
-  | BOT => BOT
-  | t1 || t2 => term_map h t1 || term_map h t2
-  | t1 (+) t2 => term_map h t1 (+) term_map h t2
-  | t1 * t2 => term_map h t1 * term_map h t2
-  | VAR x => VAR (h x)
-  | LAMBDA t1 => LAMBDA (term_map (option_map h) t1)
-  end.
-
-Fixpoint term_sub {Var Var' : Set} (h : Var -> Term Var') (t : Term Var) :
-  Term Var' :=
-  match t with
-  | TOP => TOP
-  | BOT => BOT
-  | t1 || t2 => term_sub h t1 || term_sub h t2
-  | t1 (+) t2 => term_sub h t1 (+) term_sub h t2
-  | t1 * t2 => term_sub h t1 * term_sub h t2
-  | VAR v => h v
-  | LAMBDA t1 => LAMBDA (term_sub (fun x => 
-    match x with
-    | None => VAR None
-    | Some y => term_map (@Some Var') (h y)
-    end) t1)
-  end.
-
-Notation "x @ f" := (term_sub f x) : term_scope.
-
-Definition beta_sub {Var : Set} (x : Term (option Var)) (y : Term Var) :
-  Term Var := x @ (fun v => match v with None => y | Some v' => VAR v' end).
+(** ** Lambda notation *)
 
 Fixpoint iter {a : Type} (z : a) (s : a -> a) (n : nat) {struct n} :=
   match n with
@@ -111,7 +73,6 @@ Definition var_ {Var : Set} (n : nat) : Term (option_ n Var) :=
   @VAR (option_ n Var) (iter_dep (@None' Var) Some' n).
 *)
 
-
 Section I.
   Definition v0 {Var : Set} : Term (option_ 1 Var) := VAR None.
   Definition v1 {Var : Set} : Term (option_ 2 Var) := VAR (Some None).
@@ -131,7 +92,6 @@ Section I.
 End I.
 Print S.  (* Ugly! *)
 
-
 Notation "x 'o' y" := (B * x * y) : term_scope.
 
 Definition term_join {Var : Set} x y : Term Var := x || y.
@@ -139,447 +99,3 @@ Definition term_join {Var : Set} x y : Term Var := x || y.
 (* TODO figure out how to use lambda notation
 Notation "\ x , y" := (LAMBDA) : code_scope.
 *)
-
-(** ** Reduction relations *)
-
-Inductive star {Var : Set} (r : relation (Term Var)) : relation (Term Var) :=
-  | star_step {x y} : r x y -> star r x y
-  | star_refl {x} : star r x x
-  | star_trans {x} y {z} : star r x y -> star r y z -> star r x z.
-Hint Constructors star.
-
-Inductive weak_star
-  {Var : Set} (r : relation (Term Var)) : relation (Term Var) :=
-  | weak_star_refl {x} : weak_star r x x
-  | weak_star_trans {x} y {z} : r x y -> weak_star r y z -> weak_star r x z.
-Hint Constructors weak_star.
-
-Lemma weaken_star (Var : Set) (r : relation (Term Var)) (x y : Term Var) :
-  star r x y <-> weak_star r x y.
-Proof.
-  split; intro H; induction H; eauto.
-  clear H H0; induction IHstar1; auto.
-  apply weak_star_trans with y; auto.
-Qed.
-
-Lemma weak_star_flip (Var : Set) (r : relation (Term Var)) (x y : Term Var) :
-  weak_star (flip r) x y <-> weak_star r y x.
-Proof.
-  repeat rewrite <- weaken_star.
-  split; intro H; induction H; eauto.
-Qed.
-
-
-Inductive probe {Var : Set} : relation (Term Var) :=
-  | probe_refl {x} : probe x x
-  | probe_trans {x} y {z} : probe x y -> probe y z -> probe x z
-  | probe_top {x} : probe x (x * TOP).
-Hint Constructors probe.
-
-Inductive probe_step {Var : Set} : relation (Term Var) :=
-  | probe_step_top {x} : probe_step x (x * TOP).
-Hint Constructors probe_step.
-
-Lemma weaken_probe (Var : Set) (x y : Term Var) :
-  probe x y <-> weak_star probe_step x y.
-Proof.
-  rewrite <- weaken_star.
-  split; intro H; induction H; eauto.
-  inversion H; auto.
-Qed.
-
-Inductive beta {Var : Set} : relation (Term Var) :=
-  | beta_refl {x} : beta x x
-  | beta_trans {x} y {z} : beta x y -> beta y z -> beta x z
-  | beta_left {x x' y} : beta x x' -> beta (x * y) (x' * y)
-  | beta_right {x y y'} : beta y y' -> beta (x * y) (x * y')
-  | beta_lam {x y} : beta (LAMBDA x * y) (beta_sub x y)
-  | beta_j_ap {x y z} : beta ((x || y) * z) (x * z || y * z)
-  | beta_r_ap {x y z} : beta ((x (+) y) * z) (x * z (+) y * z)
-  | beta_r_idem {x} : beta (x (+) x) x
-  | beta_r_sym {x y} : beta (x (+) y) (y (+) x)
-  | beta_r_sym_sym {w x y z} :
-      beta ((w(+)x) (+) (y(+)z)) ((x(+)y) (+) (z(+)w)).
-Hint Constructors beta.
-
-Inductive beta_step {Var : Set} : relation (Term Var) :=
-  | beta_step_left {x x' y} : beta_step x x' -> beta_step (x * y) (x' * y)
-  | beta_step_right {x y y'} : beta_step y y' -> beta_step (x * y) (x * y')
-  | beta_step_lam {x y} : beta_step (LAMBDA x * y) (beta_sub x y)
-  | beta_step_j_ap {x y z} : beta_step ((x || y) * z) (x * z || y * z)
-  | beta_step_r_ap {x y z} : beta_step ((x (+) y) * z) (x * z (+) y * z)
-  | beta_step_r_idem {x} : beta_step (x (+) x) x
-  | beta_step_r_sym {x y} : beta_step (x (+) y) (y (+) x)
-  | beta_step_r_sym_sym {w x y z} :
-      beta_step ((w(+)x) (+) (y(+)z)) ((x(+)y) (+) (z(+)w)).
-Hint Constructors beta_step.
-
-Lemma weaken_beta (Var : Set) (x y : Term Var) :
-  beta x y <-> weak_star beta_step x y.
-Proof.
-  rewrite <- weaken_star.
-  split; intro H; induction H; eauto.
-  - clear H; induction IHbeta; eauto.
-  - clear H; induction IHbeta; eauto.
-  - induction H; auto.
-Qed.
-
-
-Inductive pi {Var : Set} : relation (Term Var) :=
-  | pi_refl {x} : pi x x
-  | pi_trans {x} y {z} : pi x y -> pi y z -> pi x z
-  | pi_left {x x' y} : pi x x' -> pi (x * y) (x' * y)
-  | pi_right {x y y'} : pi y y' -> pi (x * y) (x * y')
-  | pi_lam {x y} : pi (LAMBDA x * y) (beta_sub x y)
-  | pi_j_ap {x y z} : pi ((x || y) * z) (x * z || y * z)
-  | pi_r_ap {x y z} : pi ((x (+) y) * z) (x * z (+) y * z)
-  | pi_r_idem {x} : pi (x (+) x) x
-  | pi_r_sym {x y} : pi (x (+) y) (y (+) x)
-  | pi_r_sym_sym {w x y z} :
-      pi ((w(+)x) (+) (y(+)z)) ((x(+)y) (+) (z(+)w))
-  | pi_top x : pi TOP x
-  | pi_bot x : pi x BOT
-  | pi_j_left {x y} : pi (x || y) x
-  | pi_j_right {x y} : pi (x || y) y.
-Hint Constructors pi.
-
-Inductive pi_step {Var : Set} : relation (Term Var) :=
-  | pi_step_left {x x' y} : pi_step x x' -> pi_step (x * y) (x' * y)
-  | pi_step_right {x y y'} : pi_step y y' -> pi_step (x * y) (x * y')
-  | pi_step_lam {x y} : pi_step (LAMBDA x * y) (beta_sub x y)
-  | pi_step_j_ap {x y z} : pi_step ((x || y) * z) (x * z || y * z)
-  | pi_step_r_ap {x y z} : pi_step ((x (+) y) * z) (x * z (+) y * z)
-  | pi_step_r_idem {x} : pi_step (x (+) x) x
-  | pi_step_r_sym {x y} : pi_step (x (+) y) (y (+) x)
-  | pi_step_r_sym_sym {w x y z} :
-      pi_step ((w(+)x) (+) (y(+)z)) ((x(+)y) (+) (z(+)w))
-  | pi_step_top x : pi_step TOP x
-  | pi_step_bot x : pi_step x BOT
-  | pi_step_j_left {x y} : pi_step (x || y) x
-  | pi_step_j_right {x y} : pi_step (x || y) y.
-Hint Constructors pi_step.
-
-Lemma weaken_pi (Var : Set) (x y : Term Var) :
-  pi x y <-> weak_star pi_step x y.
-Proof.
-  rewrite <- weaken_star.
-  split; intro H; induction H; eauto.
-  - clear H; induction IHpi; eauto.
-  - clear H; induction IHpi; eauto.
-  - induction H; auto.
-Qed.
-
-
-Hint Rewrite @beta_j_ap @beta_r_ap @beta_r_idem : beta_safe.
-Hint Rewrite @beta_lam : beta_unsafe.
-
-Tactic Notation "beta_simpl" :=
-  autorewrite with beta_safe.
-Tactic Notation "beta_simpl" "in" hyp(H) :=
-  autorewrite with beta_safe in H.
-Tactic Notation "beta_reduce" :=
-  autorewrite with beta_safe beta_unsafe.
-Tactic Notation "beta_reduce" "in" hyp(H) :=
-  autorewrite with beta_safe beta_unsafe in H.
-Tactic Notation "term_simpl" :=
-  autorewrite with beta_safe term_simpl.
-Tactic Notation "term_simpl" "in" hyp(H) :=
-  autorewrite with beta_safe term_simpl in H.
-
-(** To avoid nontermination in [beta_reduce],
-    we provide a mechanism to "freeze" terms during reduction. *)
-Tactic Notation "freeze" reference(c) "in" tactic(tac) :=
-  let v := fresh "v" in
-  let H := fresh "Hv" in
-  assert (exists v, c=v) as H;
-  [ exists c; reflexivity
-  | destruct H as [v H]; rewrite H; tac; destruct H].
-
-
-Class Commuting (Var : Set) (r s : relation (Term Var)) :=
-  commuting : forall x y z, r x y -> s y z -> exists y', s x y' /\ r y' z.
-
-Tactic Notation
-  "commute" ident(x) ident(y) ident(z) constr(xy) constr(yz)
-  "as" ident(w) :=
-  let xy := fresh x y in
-  let yx := fresh y x in
-  let yz := fresh y z in
-  let zy := fresh z y in
-  let xw := fresh x w in
-  let wz := fresh w z in
-  let H := fresh in
-  match type of xy with
-    | ?r y x => assert (flip r x y) as xy; [unfold flip; assumption | idtac]
-    | ?r x y => idtac
-  end;
-  match type of yz with
-    | ?r z y => assert (flip r y z) as yz; [unfold flip; assumption | idtac]
-    | ?r y z => idtac
-  end;
-  set (H := commuting x y z xy yz);
-  destruct H as [w [xw wz]];
-  try unfold flip in xw, wz.
-
-Lemma weaken_commuting (Var : Set) (r s r' s' : relation (Term Var)) :
-  (forall (x y : Term Var), r x y <-> weak_star r' x y) ->
-  (forall (x y : Term Var), s x y <-> weak_star s' x y) ->
-  (forall x y z, r' x y -> s' y z -> exists y', s x y' /\ r y' z) ->
-  Commuting Var r s.
-Proof.
-  intros Hr Hs Hweak x y z rxy syz.
-  rewrite Hr in rxy.
-  rewrite Hs in syz.
-  induction rxy; induction syz; eauto.
-  - exists x; rewrite Hr, Hs; auto.
-  - exists z; rewrite Hr, Hs; split; auto.
-    apply weak_star_trans with y; auto.
-  - exists x; rewrite Hr, Hs; split; auto.
-    apply weak_star_trans with y; auto.
-  - admit. (* TODO also assume r == star r and s == star s,
-              then use strong induction *)
-Qed.
-
-
-Instance probe_reflexive (Var : Set) : Reflexive (@probe Var).
-Proof.
-  auto.
-Qed.
-
-Instance probe_transitive (Var : Set) : Transitive (@probe Var).
-Proof.
-  intros x y z; apply probe_trans.
-Qed.
-
-Instance probe_preorder (Var : Set) : PreOrder (@probe Var).
-Proof.
-  split; [apply probe_reflexive | apply probe_transitive].
-Qed.
-
-Lemma probe_step_probe (Var : Set) (x y : Term Var) :
-  probe_step x y -> probe x y.
-Proof.
-  intro H; inversion H; auto.
-Qed.
-
-Ltac simpl_probe_step :=
-  repeat
-  match goal with
-    | [H : probe_step _ _ |- _] => destruct H
-  (*
-    | [|- probe ?x ?y] => rewrite weaken_probe
-    | [H : star probe_step _ _ |- _] => induction H
-  *)
-    | [H : probe_step ?x ?x -> _ |- _] => clear H
-  end;
-  eauto.
-
-Instance commuting_flip_probe_probe (Var : Set) :
-  Commuting Var (flip probe) probe.
-Proof.
-  apply (weaken_commuting _ _ _ (flip probe_step) probe_step); auto.
-  - intros x y; rewrite weak_star_flip; compute; apply weaken_probe.
-  - apply weaken_probe.
-  - unfold flip; intros x y z xy yz.
-    induction xy; induction yz; eauto.
-Qed.
-
-
-Instance beta_reflexive (Var : Set) : Reflexive (@beta Var).
-Proof.
-  auto.
-Qed.
-
-Instance beta_transitive (Var : Set) : Transitive (@beta Var).
-Proof.
-  intros x y z; apply beta_trans.
-Qed.
-
-Instance beta_preorder (Var : Set) : PreOrder (@beta Var).
-Proof.
-  split; [apply beta_reflexive | apply beta_transitive].
-Qed.
-
-Instance beta_step_subrelation (Var : Set) :
-  (@subrelation (Term Var)) beta_step beta.
-Proof.
-  intros x y H; induction H; eauto.
-Qed.
-
-Instance APP_beta (Var : Set) :
-  Proper (beta ==> beta ==> beta) (@APP Var).
-Proof.
-  intros x x' Hx y y' Hy; transitivity (x * y'); auto.
-Qed.
-
-Ltac simpl_beta_step :=
-  (* repeat *)
-  match goal with
-    | [H : beta_step _ _ |- _] => induction H
-    | [H : beta_step ?x ?x -> _ |- _] => clear H
-  end.
-
-Lemma beta_step_beta (Var : Set) (x y : Term Var) :
-  beta_step x y -> beta x y.
-Proof.
-  intro H; induction H; auto.
-Qed.
-
-Instance commuting_flip_beta_beta (Var : Set) : Commuting Var (flip beta) beta.
-Proof.
-  apply (weaken_commuting _ _ _ (flip beta_step) beta_step); auto.
-  - intros x y; rewrite weak_star_flip; compute; apply weaken_beta.
-  - apply weaken_beta.
-  - compute; intros x y z xy yz.
-    induction xy; induction yz; auto.
-    (* TODO try induction over just one variable,
-       mapping beta to beta.
-       The only problem is with steps that are the same (use refl)
-       and in beta_r_ when redexes intersect.
-       Try to write a tactic matching against beta constructors. *)
-Admitted. 
-
-Instance commuting_flip_beta_probe (Var : Set) :
-  Commuting Var (flip beta) probe.
-Proof.
-  apply (weaken_commuting _ _ _ (flip beta_step) probe_step); auto.
-  - intros x y; rewrite weak_star_flip; compute; apply weaken_beta.
-  - apply weaken_probe.
-  - compute; intros x y z xy yz.
-    destruct yz.
-    exists (x * TOP); repeat split; auto.
-    apply (@weak_star_trans _ _ x0 x x) in xy; auto.
-    rewrite <- weaken_beta in xy; auto.
-Qed.
-
-Instance commuting_beta_probe (Var : Set) : Commuting Var beta probe.
-Proof.
-  apply (weaken_commuting _ _ _ beta_step probe_step); auto.
-  - apply weaken_beta.
-  - apply weaken_probe.
-  - compute; intros x y z xy yz; destruct yz; exists (x * TOP); split; auto.
-    rewrite xy; reflexivity.
-Qed.
-
-
-Instance pi_reflexive (Var : Set) : Reflexive (@pi Var).
-Proof.
-  auto.
-Qed.
-
-Instance pi_transitive (Var : Set) : Transitive (@pi Var).
-Proof.
-  intros x y z; apply pi_trans.
-Qed.
-
-Instance pi_preorder (Var : Set) : PreOrder (@pi Var).
-Proof.
-  split; [apply pi_reflexive | apply pi_transitive].
-Qed.
-
-Instance pi_step_pi_subrelation (Var : Set) :
-  (@subrelation (Term Var)) pi_step pi.
-Proof.
-  intros x y H; induction H; eauto.
-Qed.
-
-Instance beta_step_pi_subrelation (Var : Set) :
-  (@subrelation (Term Var)) beta_step pi.
-Proof.
-  intros x y H; induction H; eauto.
-Qed.
-
-Instance beta_pi_subrelation (Var : Set) : (@subrelation (Term Var)) beta pi.
-Proof.
-  intros x y Hb; induction Hb; eauto.
-Qed.
-
-Instance pi_proper_beta (Var : Set) : Proper (beta --> beta ++> impl) (@pi Var).
-Proof.
-  intros x x' xx' y y' yy' Hp; compute in yy'.
-  apply beta_pi_subrelation in xx'; rewrite xx'.
-  apply beta_pi_subrelation in yy'; rewrite <- yy'.
-  auto.
-Qed.
-
-Instance APP_pi (Var : Set) :
-  Proper (pi ==> pi ==> pi) (@APP Var).
-Proof.
-  intros x x' Hx y y' Hy; transitivity (x * y'); auto.
-Qed.
-
-Ltac simpl_pi_step :=
-  (* repeat *)
-  match goal with
-    | [H : pi_step _ _ |- _] => induction H
-    | [H : pi_step ?x ?x -> _ |- _] => clear H
-  end.
-
-Lemma pi_step_pi (Var : Set) (x y : Term Var) :
-  pi_step x y -> pi x y.
-Proof.
-  intro H; induction H; auto.
-Qed.
-
-Instance commuting_flip_pi_pi (Var : Set) : Commuting Var (flip pi) pi.
-Proof.
-  apply (weaken_commuting _ _ _ (flip pi_step) pi_step); auto.
-  - intros x y; rewrite weak_star_flip; compute; apply weaken_pi.
-  - apply weaken_pi.
-  - compute; intros x y z xy yz.
-    induction xy; induction yz; auto.
-    (* TODO similar to commuting_flip_beta_beta *)
-Admitted. 
-
-Instance commuting_flip_pi_probe (Var : Set) :
-  Commuting Var (flip pi) probe.
-Proof.
-  apply (weaken_commuting _ _ _ (flip pi_step) probe_step); auto.
-  - intros x y; rewrite weak_star_flip; compute; apply weaken_pi.
-  - apply weaken_probe.
-  - compute; intros x y z xy yz.
-    destruct yz.
-    exists (x * TOP); repeat split; auto.
-    apply (@weak_star_trans _ _ x0 x x) in xy; auto.
-    rewrite <- weaken_pi in xy; auto.
-Qed.
-
-Instance commuting_pi_probe (Var : Set) : Commuting Var pi probe.
-Proof.
-  apply (weaken_commuting _ _ _ pi_step probe_step); auto.
-  - apply weaken_pi.
-  - apply weaken_probe.
-  - compute; intros x y z xy yz; destruct yz; exists (x * TOP); split; auto.
-    rewrite xy; reflexivity.
-Qed.
-
-(* TODO try to replace this with commuting_beta_step_pi
-   since [beta TOP x -> x == TOP]? *)
-Lemma beta_step_pi_top (Var : Set) (x y : Term Var) :
-  beta_step x y -> (pi x TOP <-> pi y TOP).
-Proof.
-  intro Hb; split; intro Hp.
-  - admit. (* TODO similar strategy to commuting_flip_beta_beta *)
-  - rewrite Hb; auto.
-Qed.
-
-Lemma beta_pi_top (Var : Set) (x y : Term Var) :
-  beta x y -> (pi x TOP <-> pi y TOP).
-Proof.
-  intro Hb; rewrite weaken_beta in Hb; induction Hb; try tauto.
-  transitivity (pi y TOP); auto.
-  apply beta_step_pi_top; auto.
-Qed.
-
-Lemma probe_pi_top (Var : Set) (x y : Term Var) :
-  probe x y -> pi x TOP -> pi y TOP.
-Proof.
-  intro Hp; rewrite weaken_probe in Hp; induction Hp; try tauto.
-  destruct H; intro H; apply IHHp.
-  transitivity (TOP * TOP : Term Var); auto.
-  transitivity (K * TOP * TOP : Term Var); auto.
-  unfold K.
-  rewrite beta_lam; compute.
-  rewrite beta_lam; compute.
-  auto.
-Qed.
