sandbox/combinators/InformationOrdering.v
@@ -1,0 +1,610 @@
+(** * Information ordering and observable equivalence *)
+
+Require Import Coq.Logic.Classical_Prop.
+Require Import Coq.Program.Basics.
+Require Import Coq.Program.Equality.
+Require Import Coq.Setoids.Setoid.
+Require Import Coq.Classes.RelationClasses.
+Require Import Coq.Classes.Morphisms.
+Require Import Coq.Lists.List.
+Require Export Convergence.
+Open Scope code_scope.
+
+Definition code_le {Var : Set} (x y : Code Var) :=
+  forall (Var' : Set) (c : Code Var') (f : Var -> Code Var'),
+  conv (c * (x @ f)) -> conv (c * (y @ f)).
+Notation "x [= y" := (code_le x y) : code_scope.
+
+Definition code_eq {Var : Set} (x y : Code Var) := x [= y /\ y [= x.
+Notation "x == y" := (code_eq x y) : code_scope.
+
+Instance code_le_eq_subrelation (Var : Set) :
+  subrelation (@code_eq Var) (@code_le Var).
+Proof.
+  unfold subrelation, predicate_implication, pointwise_lifting.
+  unfold code_eq; intros x y [xy yx]; auto.
+Qed.
+
+Instance code_le_beta_proper (Var : Set) :
+  Proper (beta ==> beta ==> iff) (@code_le Var).
+Proof.
+  intros x x' Hx y y' Hy; split; unfold code_le; intros Hle Var' c f Hc.
+    rewrite <- Hy; apply Hle; rewrite -> Hx; auto.
+  rewrite -> Hy; apply Hle; rewrite <- Hx; auto.
+Qed.
+
+Instance code_eq_beta_proper (Var : Set) :
+  Proper (beta ==> beta ==> iff) (@code_eq Var).
+Proof.
+  unfold code_eq.
+  intros x x' xx' y y' yy'; split; intros [xy yx].
+    split; rewrite <- xx'; rewrite <- yy'; auto.
+  split; rewrite -> xx'; rewrite -> yy'; auto.
+Qed.
+
+Lemma code_le_beta (Var : Set) (x y : Code Var) : beta x y -> x [= y.
+Proof.
+  unfold code_le; intros H Var' c f Hc.
+  rewrite <- H; auto.
+Qed.
+Hint Resolve code_le_beta.
+
+Instance code_le_beta_subrelation (Var : Set) :
+  subrelation beta (@code_le Var).
+Proof.
+  intros x y H; apply code_le_beta; auto.
+Qed.
+
+Lemma code_eq_beta (Var : Set) (x y : Code Var) : beta x y -> x == y.
+Proof.
+  unfold code_le; intro H; split; intros Var' c f Hc.
+  rewrite <- H; auto.
+  rewrite -> H; auto.
+Qed.
+Hint Resolve code_eq_beta.
+
+Instance code_eq_beta_subrelation (Var : Set) :
+  subrelation beta (@code_eq Var).
+Proof.
+  simpl_relation; apply code_eq_beta; auto.
+Qed.
+
+Instance code_le_proper_pi (Var : Set) :
+  Proper (pi ++> pi --> impl) (@code_le Var).
+Proof.
+  intros x x' Hx y y' Hy; unfold code_le; intros Hle Var' c f Hc.
+  unfold flip in *.
+  rewrite Hy.
+  apply Hle; rewrite -> Hx; auto.
+Qed.
+
+Instance code_le_pi_subrelation (Var : Set) :
+  subrelation (inverse pi) (@code_le Var).
+Proof.
+  unfold subrelation, predicate_implication, pointwise_lifting, flip.
+  intros x y H; unfold code_le; intros Var' c f Hc.
+  rewrite -> H; auto.
+Qed.
+
+Instance code_le_refl (Var : Set) : Reflexive (@code_le Var).
+Proof.
+  unfold code_le; auto.
+Qed.
+
+Instance code_eq_refl (Var : Set) : Reflexive (@code_eq Var).
+Proof.
+  simpl_relation.
+Qed.
+
+Instance code_le_trans (Var : Set) : Transitive (@code_le Var).
+Proof.
+  unfold code_le; auto.
+Qed.
+
+Instance code_eq_trans (Var : Set) : Transitive (@code_eq Var).
+Proof.
+  unfold code_eq, code_le; simpl_relation.
+Qed.
+
+Instance code_eq_sym (Var : Set) : Symmetric (@code_eq Var).
+Proof.
+  unfold code_eq, code_le; simpl_relation.
+Qed.
+
+Instance code_le_preorder (Var : Set) : PreOrder (@code_le Var).
+Proof.
+  split; [apply code_le_refl | apply code_le_trans].
+Qed.
+
+Instance code_eq_equivalence (Var : Set) : Equivalence (@code_eq Var).
+Proof.
+  split; [apply code_eq_refl | apply code_eq_sym | apply code_eq_trans].
+Qed.
+
+Instance code_le_partialorder (Var : Set) :
+  PartialOrder (@code_eq Var) (@code_le Var).
+Proof.
+  simpl_relation.
+Qed.
+
+Lemma code_le_ap_right (Var : Set) (x y y' : Code Var) :
+  y [= y' -> x * y [= x * y'.
+Proof.
+  unfold code_le; intros H Var' c f.
+  repeat rewrite code_sub_ap.
+  intros Hconv.
+  rewrite <- beta_b.
+  apply H.
+  rewrite -> beta_b.
+  auto.
+Qed.
+Hint Resolve code_le_ap_right.
+
+Lemma code_le_ap_left (Var : Set) (x x' y : Code Var) :
+  x [= x' -> x * y [= x' * y.
+Proof.
+  unfold code_le; intros H Var' c f.
+  repeat rewrite code_sub_ap.
+  intros Hconv.
+  rewrite <- (beta_right (beta_left beta_i)).
+  rewrite <- (beta_right beta_c).
+  rewrite <- beta_b.
+  apply H.
+  rewrite -> beta_b.
+  rewrite -> (beta_right beta_c).
+  rewrite -> (beta_right (beta_left beta_i)).
+  auto.
+Qed.
+Hint Resolve code_le_ap_left.
+
+Lemma code_le_ap (Var : Set) (x x' y y' : Code Var) :
+  x [= x' -> y [= y' -> x * y [= x' * y'.
+Proof.
+  intros Hx Hy; transitivity (x * y'); auto.
+Qed.
+Hint Resolve code_le_ap.
+
+Lemma code_eq_ap_right (Var : Set) (x y y' : Code Var) :
+  y == y' -> x * y == x * y'.
+Proof.
+  unfold code_eq; intros [H H']; split; auto.
+Qed.
+Hint Resolve code_eq_ap_right.
+
+Lemma code_eq_ap_left (Var : Set) (x x' y : Code Var) :
+  x == x' -> x * y == x' * y.
+Proof.
+  unfold code_eq; intros [H H']; split; auto.
+Qed.
+Hint Resolve code_eq_ap_left.
+
+Lemma code_eq_ap (Var : Set) (x x' y y' : Code Var) :
+  x == x' -> y == y' -> x * y == x' * y'.
+Proof.
+  intros Hx Hy; transitivity (x * y'); auto.
+Qed.
+Hint Resolve code_eq_ap.
+
+Instance code_ap_le (Var : Set) :
+  Proper (code_le ==> code_le ==> code_le) (@code_ap Var).
+Proof.
+  intros x x' Hx y y' Hy.
+  apply code_le_trans with (x * y'); auto.
+Qed.
+
+Instance code_ap_eq (Var : Set) :
+  Proper (code_eq ==> code_eq ==> code_eq) (@code_ap Var).
+Proof.
+  intros x x' Hx y y' Hy.
+  apply code_eq_trans with (x * y'); auto.
+Qed.
+
+Ltac code_le_monotonicity := repeat ((
+  apply code_le_ap_left ||
+  apply code_le_ap_right ||
+  apply code_le_ap) ; auto).
+
+Ltac code_eq_monotonicity := repeat (
+  apply code_eq_ap_left ||
+  apply code_eq_ap_right ||
+  apply code_eq_ap).
+
+Ltac monotonicity :=
+  match goal with
+  | [|- _ [= _] => code_le_monotonicity
+  | [|- _ == _] => code_eq_monotonicity
+  end.
+
+Instance conv_proper_le (Var : Set) : Proper (code_le ++> impl) (@conv Var).
+Proof.
+  intros x y Hxy Hc; unfold code_le in Hxy.
+  rewrite <- var_monad_unit_right; rewrite <- beta_i.
+  apply Hxy; code_simpl; auto.
+Qed.
+
+Instance conv_proper_eq (Var : Set) : Proper (code_eq ==> iff) (@conv Var).
+Proof.
+  intros x y [Hxy Hyx]; split; intro Hc;
+  [rewrite <- Hxy | rewrite <- Hyx]; auto.
+Qed.
+
+Lemma code_sub_le_left
+  (Var Var' : Set) (f g : Var -> Code Var') (x : Code Var) :
+  (forall v, f v [= g v) -> x @ f [= x @ g.
+Proof.
+  induction x; simpl; auto.
+Qed.
+
+Lemma code_sub_le_right
+  (Var Var' : Set) (f : Var -> Code Var') (x y : Code Var) :
+  x [= y -> x @ f [= y @ f.
+Proof.
+  intros H Var'' c f'; repeat rewrite var_monad_assoc; auto.
+Qed.
+
+Instance code_sub_proper_le (Var Var' : Set) :
+  Proper ((eq ==> code_le) ==> code_le ==> code_le) (@code_sub Var Var').
+Proof.
+  intros f g Hfg x y Hxy; transitivity (y @ f);
+  [apply code_sub_le_right | apply code_sub_le_left]; auto.
+Qed.
+
+Lemma code_sub_le {Var Var' : Set} (f : Var -> Code Var') (x y : Code Var) :
+  x [= y -> x @ f [= y @ f.
+Proof.
+  intro xy; rewrite xy; reflexivity.
+Qed.
+
+Instance code_sub_proper_eq (Var Var' : Set) :
+  Proper ((eq ==> code_eq) ==> code_eq ==> code_eq) (@code_sub Var Var').
+Proof.
+  intros f g Hfg x y Hxy; transitivity (y @ f); split.
+  - rewrite Hxy; auto.
+  - rewrite <- Hxy; auto.
+  - rewrite Hfg; auto.
+  - rewrite <- Hfg; auto.
+Qed.
+
+Lemma code_sub_eq {Var Var' : Set} (f : Var -> Code Var') (x y : Code Var) :
+  x == y -> x @ f == y @ f.
+Proof.
+  intro xy; rewrite xy; reflexivity.
+Qed.
+
+Lemma code_le_top (Var : Set) (x : Code Var) : x [= TOP.
+Proof.
+  intros; rewrite (pi_top x); auto.
+Qed.
+Hint Resolve code_le_top.
+
+Lemma code_le_bot (Var : Set) (x : Code Var) : BOT [= x.
+Proof.
+  unfold code_le; intros Var' c f Hred.
+  simpl in Hred.
+  rewrite -> (pi_right (pi_bot _)).
+  auto.
+Qed.
+Hint Resolve code_le_bot.
+
+Lemma absolute_consistency (Var : Set) : ~ TOP [= (BOT : Code Var).
+Proof.
+  intro H; unfold code_le in H.
+  apply (@not_conv_bot Var).
+  rewrite <- beta_i; rewrite <- var_monad_unit_right.
+  apply H; code_simpl; auto.
+Qed.
+Hint Resolve absolute_consistency.
+
+(** ** Basic properties of information ordering *)
+
+Lemma code_le_j_left (Var : Set) (x y : Code Var) : x [= x || y.
+Proof.
+  unfold code_le; intros Var' c f Hred.
+  rewrite pi_j_left; auto.
+Qed.
+Hint Resolve code_le_j_left.
+
+Lemma code_le_j_right (Var : Set) (x y : Code Var) : y [= x || y.
+Proof.
+  unfold code_le; intros Var' c f Hred.
+  rewrite pi_j_right; auto.
+Qed.
+Hint Resolve code_le_j_right.
+
+Lemma code_le_j_ub (Var : Set) (x y z : Code Var) :
+  x [= z -> y [= z -> x || y [= z.
+Proof.
+  unfold code_le; intros Hx Hy Var' c f Hc.
+Admitted.
+Hint Resolve code_le_j_ub.
+
+Lemma code_le_join (Var : Set) (x y z : Code Var) :
+  x || y [= z <-> x [= z /\ y [= z.
+Proof.
+  split; intro H.
+    split; apply code_le_trans with (x || y); auto.
+  destruct H as [Hx Hy]; auto.
+Qed.
+Hint Resolve code_le_join.
+
+Lemma code_le_eq_j (Var : Set) (x y : Code Var) : x [= y <-> y == y || x.
+Proof.
+  split; intro H; [split | rewrite H]; auto.
+Qed.
+
+Lemma code_le_j_idem (Var : Set) (x : Code Var) : x||x [= x.
+Proof.
+  apply code_le_join; split; reflexivity.
+Qed.
+Hint Resolve code_le_j_idem.
+
+Lemma code_eq_j_idem (Var : Set) (x : Code Var) : x||x == x.
+Proof.
+  split; auto.
+Qed.
+Hint Resolve code_eq_j_idem.
+
+Lemma code_le_j_sym (Var : Set) (x y : Code Var) : x||y == y||x.
+Proof.
+  split; auto.
+Qed.
+
+Lemma code_eq_j_assoc (Var : Set) (x y z : Code Var) : x||(y||z) == (x||y)||z.
+Proof.
+  split; auto.
+    apply code_le_j_ub; auto.
+    transitivity (x||y); auto.
+  apply code_le_j_ub; auto.
+  transitivity (y||z); auto.
+Qed.
+
+Lemma code_le_j_ap_right (Var : Set) (f x y : Code Var) :
+  f * x || f * y [= f * (x || y).
+Proof.
+  apply code_le_join; split; monotonicity.
+Qed.
+
+Lemma code_le_j_bot_left (Var : Set) (x : Code Var) : BOT || x == x.
+Proof.
+  split; auto.
+Qed.
+Hint Rewrite code_le_j_bot_left : code_simpl.
+
+Lemma code_le_j_bot_right (Var : Set) (x : Code Var) : x || BOT == x.
+Proof.
+  split; auto.
+Qed.
+Hint Rewrite code_le_j_bot_right : code_simpl.
+
+Lemma code_le_j_top_left (Var : Set) (x : Code Var) : TOP || x == TOP.
+Proof.
+  split; auto.
+Qed.
+Hint Rewrite code_le_j_top_left : code_simpl.
+
+Lemma code_le_j_top_right (Var : Set) (x : Code Var) : x || TOP == TOP.
+Proof.
+  split; auto.
+Qed.
+Hint Rewrite code_le_j_top_right : code_simpl.
+
+(** ** Reasoning with extensionality *)
+
+(*
+Ltac abstract M x :=
+  match m with
+  | x => code_ap code_i x
+  | code_ap ?M1 ?M2 =>
+    let code_ap N1 _ := abstract M1 x in
+    let code_ap N2 _ := abstract M2 x in
+    code_ap (code_ap (code_ap code_s N1) N2) x
+  | _ => code_ap code_k x
+  end.
+
+Ltac beta_subs :=
+  match goal with
+  | beta x y
+*)
+
+Lemma code_le_extensionality (Var : Set) (x x' : Code Var) :
+  (forall y, x * y [= x' * y) -> x [= x'.
+Proof.
+  unfold code_le; intros H Var' c f Hconv.
+  (* TODO implement via abstraction algorithm *)
+Admitted.
+
+Lemma code_eq_extensionality (Var : Set) (x x' : Code Var) :
+  (forall y, x * y == x' * y) -> x == x'.
+Proof.
+  intro H; split; apply code_le_extensionality; apply H.
+Qed.
+
+Tactic Notation "eta_expand" :=
+  let x := fresh in
+  match goal with
+  | [|- _ [= _] => apply code_le_extensionality; intro x
+  | [|- _ == _] => apply code_eq_extensionality; intro x
+  end.
+
+Tactic Notation "eta_expand" "as" ident(x) :=
+  match goal with
+  | [|- _ [= _] => apply code_le_extensionality; intro x
+  | [|- _ == _] => apply code_eq_extensionality; intro x
+  end.
+
+Tactic Notation "eta_expand" "in" hyp(H) :=
+  eapply code_le_ap_left in H; beta_reduce in H.
+
+Ltac beta_eta :=
+  beta_reduce; auto
+  || eta_expand; beta_reduce; auto
+  || eta_expand; eta_expand; beta_reduce; auto
+  || eta_expand; eta_expand; eta_expand; beta_reduce; auto.
+
+Lemma code_eq_ap_top (Var : Set) (x : Code Var) : TOP * x == TOP.
+Proof.
+  split; auto.
+  rewrite (pi_top (K * TOP : Code Var)) at 2; beta_simpl; auto.
+Qed.
+Hint Rewrite code_eq_ap_top : code_simpl.
+
+Lemma code_eq_b_i (Var : Set) (x : Code Var) : I o x == x.
+Proof.
+  beta_eta.
+Qed.
+Hint Rewrite code_eq_b_i : code_simpl.
+
+Lemma code_eq_c_b_i (Var : Set) (x : Code Var) : x o I == x.
+Proof.
+  beta_eta.
+Qed.
+Hint Rewrite code_eq_b_i : code_simpl.
+
+Lemma code_eq_s_k_b (Var : Set) (x : Code Var) : S * (K * x) == B * x.
+Proof.
+  beta_eta.
+Qed.
+Hint Rewrite code_eq_s_k_b : code_simpl.
+
+Lemma code_eq_s_k_c (Var : Set) (x y : Code Var) :
+  S * x * (K * y) == C * x * y.
+Proof.
+  beta_eta.
+Qed.
+Hint Rewrite code_eq_s_k_c : code_simpl.
+
+(** We will use classical reasoning for case analysis. *)
+
+Lemma case_le (Var : Set) (x y : Code Var) (p : Prop) :
+  (x [= y -> p) -> (~ x [= y -> p) -> p.
+Proof.
+  intros H H'; elim (classic (x [= y)); auto.
+Qed.
+
+Tactic Notation "case_le" constr(xy) :=
+  match xy with
+  | ?x [= ?y => apply (@case_le _ x y _)
+  end; intro.
+
+Tactic Notation "case_le" constr(xy) "as" ident(H) :=
+  match xy with
+  | ?x [= ?y => apply (@case_le _ x y _)
+  end; intro H.
+
+(** ** Simpler versions of convergence and ordering  *)
+
+Fixpoint code_apply {Var : Set} (x : Code Var) (ys : list (Code Var)) :
+  Code Var :=
+  match ys with
+  | nil => x
+  | (y ::ys')%list => code_apply (x * y) ys'
+  end.
+
+Notation "x ** y" := (code_apply x y) : code_scope.
+
+Instance code_apply_proper_le (Var : Set) :
+  Proper (code_le ==> eq ==> code_le) (@code_apply Var).
+Proof.
+  intros x x' xx' y y' yy'; subst.
+  revert x x' xx'; induction y'; simpl; auto.
+Qed.
+
+Instance code_apply_proper_eq (Var : Set) :
+  Proper (code_eq ==> eq ==> code_eq) (@code_apply Var).
+Proof.
+  intros x x' [xx' x'x] y y' yy'; subst; split;
+  [rewrite xx' | rewrite x'x]; auto.
+Qed.
+
+Fixpoint code_repeat {Var : Set} (x : Code Var) (n : nat) : list (Code Var) :=
+  match n with
+  | 0 => nil
+  | Succ n' => (x :: code_repeat x n')%list
+  end.
+
+Notation "x ^^ n" := (code_repeat x n) : code_scope.
+
+Fixpoint code_tuple {Var : Set} (ys : list (Code Var)) : Code Var :=
+  match ys with
+  | nil => I
+  | (y :: ys')%list => code_tuple ys' o (C * I * y)
+  end.
+
+Lemma beta_tuple_apply (Var : Set) (ys : list (Code Var)) :
+  forall x : Code Var, beta (code_tuple ys * x) (x ** ys).
+Proof.
+  induction ys; simpl; auto; intro x.
+  beta_simpl; auto.
+Qed.
+Hint Resolve beta_tuple_apply.
+
+Instance code_tuple_le (Var : Set) :
+  Proper (Forall2 code_le ==> code_le) (@code_tuple Var).
+Proof.
+  intros xs xs' xsxs'; induction xsxs'; simpl; auto.
+Qed.
+
+Lemma code_repeat_commute_1 (Var : Set) (x y : Code Var) (n : nat) :
+  (x * y) ** y ^^ n = (x ** y ^^ n) * y.
+Proof.
+  revert x y; induction n; simpl; auto.
+Qed.
+
+Lemma code_repeat_top (Var : Set) (ys : list (Code Var)) :
+  Forall2 code_le ys (TOP ^^ length ys).
+Proof.
+  induction ys; simpl; auto.
+Qed.
+Hint Resolve code_repeat_top.
+
+Lemma ap_top_conv (Var : Set) (x : Code Var) : conv x <-> conv (x * TOP).
+Proof.
+  assert (probe x (x * TOP)) as eq; auto.
+  rewrite <- eq; reflexivity.
+Qed.
+
+Definition weak_code_le {Var : Set} (x x' : Code Var) : Prop :=
+  forall (ys : list (Code Empty_set)) (f : Var -> Code Empty_set),
+  conv ((x @ f) ** ys) -> conv ((x' @ f) ** ys).
+
+Lemma weak_code_le_complete (Var : Set) (x x' : Code Var) :
+  x [= x' -> weak_code_le x x'.
+Proof.
+  unfold code_le; intros H ys f Hconv.
+  rewrite <- beta_tuple_apply; apply H.
+  rewrite beta_tuple_apply; auto.
+Qed.
+
+Lemma weak_code_le_sound (Var : Set) (x x' : Code Var) :
+  weak_code_le x x' -> x [= x'.
+Proof.
+  unfold code_le; intros H Var' c f Hconv.
+  assert (forall (ys : list (Code Var')),
+    conv ((x @ f) ** ys) -> conv ((x' @ f) ** ys)) as H'; auto; clear H.
+  set (y := x @ f) in *; set (y' := x' @ f) in *.
+  inversion Hconv; simpl; auto.
+  (* TODO maybe prove by induction on BT of c? *)
+Admitted.
+
+Theorem code_le_weaken (Var : Set) (x x' : Code Var) :
+  x [= x' <-> weak_code_le x x'.
+Proof.
+  split; [apply weak_code_le_complete | apply weak_code_le_sound].
+Qed.
+
+Ltac code_le_weaken := apply code_le_weaken; unfold weak_code_le.
+
+Lemma conv_ap (Var : Set) (x a : Code Var) : conv (x * a) -> conv x.
+Proof.
+  rewrite (code_le_top _ a).
+  intros [y [xy yt]].
+  exists y; split; auto.
+  unfold close in xy; simpl in xy; fold (@close Var) in xy.
+  transitivity ((close x) * TOP); auto.
+Qed.
+
+Lemma conv_apply (Var : Set) (x : Code Var) (ys : list (Code Var)) :
+  conv (x ** ys) -> conv x.
+Proof.
+  revert x; induction ys; simpl; intros; eauto using conv_ap.
+Qed.
