sandbox/combinators/Substitution.v
@@ -1,0 +1,216 @@
+(** * Substitution *)
+
+Require Import Coq.Classes.Morphisms.
+Require Export Codes.
+
+Fixpoint code_sub {Var Var' : Set}
+  (f : Var -> Code Var') (x : Code Var) : Code Var' :=
+  match x with
+  | code_var v => f v
+  | l * r => (code_sub f l) * (code_sub f r)
+  | TOP => TOP
+  | BOT => BOT
+  | J => J
+  | R => R
+  | I => I
+  | K => K
+  | B => B
+  | C => C
+  | S => S
+  end.
+
+Notation "x @ f" := (code_sub f x) : code_scope.
+
+Definition sub_top {Var : Set} (v : Var) : Code Empty_set := TOP.
+Definition close {Var : Set} : Code Var -> Code Empty_set := code_sub sub_top.
+
+Lemma var_monad_unit_right (Var : Set) (x : Code Var) : x @ code_var = x.
+Proof.
+  induction x; auto.
+  unfold code_sub; fold (@code_sub Var Var).
+  rewrite IHx1; rewrite IHx2; auto.
+Qed.
+Hint Rewrite var_monad_unit_right : code_simpl.
+
+Lemma var_monad_unit_left (Var Var' : Set) (f : Var -> Code Var') x :
+  (code_var x) @ f = f x.
+Proof.
+  compute; auto.
+Qed.
+Hint Rewrite var_monad_unit_left : code_simpl.
+
+Lemma code_sub_ap (Var Var' : Set)
+  (x y : Code Var) (f : Var -> Code Var') : (x * y @ f) = (x @ f) * (y @ f).
+Proof.
+  simpl; auto.
+Qed.
+Hint Rewrite code_sub_ap : code_simpl.
+
+Lemma var_monad_assoc
+  (Var Var' Var'' : Set)
+  (f : Var -> Code Var')
+  (g : Var' -> Code Var'')
+  (x : Code Var) :
+  (x @ f) @ g = x @ (fun v => (f v) @ g).
+Proof.
+  induction x; auto.
+  repeat rewrite code_sub_ap.
+  rewrite IHx1; rewrite IHx2; auto.
+Qed.
+Hint Rewrite var_monad_assoc : code_simpl.
+
+Lemma close_idempotent (Var : Set) (x : Code Var) : close (close x) = close x.
+Proof.
+  compute; code_simpl; induction x; auto.
+Qed.
+Hint Rewrite close_idempotent : beta_simpl.
+Hint Rewrite close_idempotent : code_simpl.
+
+Lemma close_closed (x : Closed) : close x = x.
+Proof.
+  compute; code_simpl; induction x;
+  match goal with [v : Empty_set |- _] => destruct v | _ => idtac end; auto.
+  rewrite IHx1; rewrite IHx2; reflexivity.
+Qed.
+Hint Rewrite close_closed : beta_simpl.
+Hint Rewrite close_closed : code_simpl.
+
+Lemma code_sub_inverse
+  (Var : Set) (f : Var -> Code Empty_set) (x : Code Empty_set) :
+  exists y, y @ f = x.
+Proof.
+  induction x;
+  match goal with
+  | [v : Empty_set |- _] => case v
+  | [|- exists y : Code Var, _ = ?x Empty_set] => exists (@x Var); auto
+  | _ =>
+    destruct IHx1 as [y1 Hy1];
+    destruct IHx2 as [y2 Hy2];
+    exists (y1 * y2); code_simpl; subst; auto
+  end.
+Qed.
+
+Lemma code_sub_ext (Var Var' : Set)
+  (f g : Var -> Code Var') (fg : forall v, f v = g v) x :
+  x @ f = x @ g.
+Proof.
+  induction x; simpl; auto.
+  rewrite IHx1; rewrite IHx2; auto.
+Qed.
+
+Lemma code_sub_proper_probe (Var Var' : Set)
+  (f : Var -> Code Var') (x y : Code Var) :
+  probe x y -> probe (x @ f) (y @ f).
+Proof.
+  intro xy; induction xy; simpl.
+  - reflexivity.
+  - transitivity (y @ f); auto.
+  - apply probe_top; auto.
+Qed.
+
+Lemma code_sub_beta_left
+  (Var Var' : Set) (f g : Var -> Code Var') (x : Code Var) :
+  (forall v, beta (f v) (g v)) -> beta (x @ f) (x @ g).
+Proof.
+  intros fg; induction x; auto.
+    compute; auto.
+  unfold code_sub; fold (@code_sub Var Var').
+  transitivity ((x1 @ g) * (x2 @ f)); auto.
+Qed.
+Hint Resolve code_sub_beta_left.
+
+Lemma code_sub_beta_right
+  (Var Var' : Set) (f : Var -> Code Var') (x y : Code Var) :
+  beta x y -> beta (x @ f) (y @ f).
+Proof.
+  intro xy; induction xy; repeat rewrite code_sub_ap; simpl; auto.
+  transitivity (y @ f); auto.
+Qed.
+Hint Resolve code_sub_beta_right.
+
+Instance code_sub_proper_beta (Var Var' : Set) :
+  Proper ((eq ==> beta) ==> beta ==> beta) (@code_sub Var Var').
+Proof.
+  intros f g Hfg x y Hxy; transitivity (y @ f);
+  [apply code_sub_beta_right | apply code_sub_beta_left]; auto.
+Qed.
+
+Lemma code_sub_pi_left
+  (Var Var' : Set) (f g : Var -> Code Var') (x : Code Var) :
+  (forall v, pi (f v) (g v)) -> pi (x @ f) (x @ g).
+Proof.
+  intros fg; induction x; auto.
+    compute; auto.
+  unfold code_sub; fold (@code_sub Var Var').
+  rewrite IHx1; rewrite IHx2; auto.
+Qed.
+Hint Resolve code_sub_pi_left.
+
+Lemma code_sub_pi_right
+  (Var Var' : Set) (f : Var -> Code Var') (x y : Code Var) :
+  pi x y -> pi (x @ f) (y @ f).
+Proof.
+  intro xy; induction xy; repeat rewrite code_sub_ap; simpl; auto.
+  transitivity (y @ f); auto.
+Qed.
+Hint Resolve code_sub_pi_right.
+
+Instance code_sub_proper_pi (Var Var' : Set) :
+  Proper ((eq ==> pi) ==> pi ==> pi) (@code_sub Var Var').
+Proof.
+  intros f g Hfg x y Hxy; transitivity (y @ f);
+  [apply code_sub_pi_right | apply code_sub_pi_left]; auto.
+Qed.
+
+Instance code_close_proper_beta (Var : Set) :
+  Proper (beta ==> beta) (@close Var).
+Proof.
+  intros x x' xx'; apply weaken_beta in xx'; induction xx'; auto.
+  revert z xx' IHxx'; induction H; compute; code_simpl; eauto.
+Qed.
+
+Instance code_close_proper_pi (Var : Set) :
+  Proper (pi ==> pi) (@close Var).
+Proof.
+  intros x x' xx'; apply weaken_pi in xx'; induction xx'; auto.
+  revert z xx' IHxx'; induction H; compute; code_simpl; eauto.
+Qed.
+
+Lemma probe_step_close (Var : Set) (x y : Code Var) :
+  probe_step x y -> probe (close x) (close y).
+Proof.
+  intro Hb; induction Hb; compute; auto.
+Qed.
+
+Lemma probe_close (Var : Set) (x y : Code Var) :
+  probe x y -> probe (close x) (close y).
+Proof.
+  intro Hb; rewrite weaken_probe in Hb; induction Hb; auto.
+  rewrite <- IHHb; clear Hb IHHb; auto using probe_step_close.
+Qed.
+
+Lemma beta_step_close (Var : Set) (x y : Code Var) :
+  beta_step x y -> beta (close x) (close y).
+Proof.
+  intro Hb; induction Hb; compute; beta_reduce; auto.
+Qed.
+
+Lemma beta_close (Var : Set) (x y : Code Var) :
+  beta x y -> beta (close x) (close y).
+Proof.
+  intro Hb; rewrite weaken_beta in Hb; induction Hb; auto.
+  rewrite <- IHHb; clear Hb IHHb; auto using beta_step_close.
+Qed.
+
+Lemma pi_step_close (Var : Set) (x y : Code Var) :
+  pi_step x y -> pi (close x) (close y).
+Proof.
+  intro Hb; induction Hb; compute; beta_reduce; auto.
+Qed.
+
+Lemma pi_close (Var : Set) (x y : Code Var) :
+  pi x y -> pi (close x) (close y).
+Proof.
+  intro Hb; rewrite weaken_pi in Hb; induction Hb; auto.
+  rewrite <- IHHb; clear Hb IHHb; auto using pi_step_close.
+Qed.
