src/Convergence.v
@@ -1,0 +1,152 @@
+(** * Convergence *)
+
+Require Import Coq.Program.Basics.
+Require Import Coq.Setoids.Setoid.
+Require Import Coq.Classes.RelationClasses.
+Require Import Coq.Classes.Morphisms.
+Require Export Reduction.
+
+Definition conv {Var : Set} (x : Term Var) : Prop :=
+  exists y, probe (close x) y /\ pi y TOP.
+
+Lemma conv_close (Var : Set) (x : Term Var) : conv (close x) <-> conv x.
+Proof.
+  unfold conv; term_simpl; tauto.
+Qed.
+
+Lemma conv_closed (x : Closed) : conv x <-> exists y, probe x y /\ pi y TOP.
+Proof.
+  unfold conv; rewrite close_closed; reflexivity.
+Qed.
+
+Inductive prob {Var : Set} : Term Var -> Prop :=
+  | prob_top : prob TOP
+  | prob_bot : prob BOT
+  | prob_r p q : prob p -> prob q -> prob (p (+) q).
+Hint Constructors prob.
+
+Definition pconv {Var : Set} (x : Term Var) (p : Term Empty_set) : Prop :=
+  prob p /\ exists y, probe (x @ sub_top) y /\ pi y p.
+
+Ltac wlog_closed x :=
+  let cx := fresh "c" x in
+  let Ex := fresh "E" x in
+  let Hcx := fresh "H" cx in
+  rename x into cx;
+  assert (exists x, x = close cx) as Ex; [exists (close cx); reflexivity|];
+  destruct Ex as [x Ex];
+  assert (close x = x) as Hcx; [rewrite -> Ex; apply close_idempotent|];
+  repeat
+  match goal with
+    | [ H : conv x |- _] =>
+        rewrite <- conv_close in H;
+        replace (close cx) with x in H
+    | [|- conv x ] =>
+        rewrite <- conv_close;
+        replace (close cx) with x
+    | _ => idtac
+  end.
+
+Instance conv_proper_beta (Var : Set) :
+  Proper (beta ==> iff) (@conv Var).
+Proof.
+  intros x x' xx'; split; intro H;
+  wlog_closed x; wlog_closed x';
+  apply beta_close in xx'; rewrite <- Ex in xx'; rewrite <- Ex' in xx'.
+  - destruct H as [y [xy yt]].
+    rewrite <- Ex in xy.
+    commute x' x y xx' xy as y'; exists y'.
+    split; [rewrite <- Ex'; auto|].
+    rewrite <- (beta_pi_top _ _ _ y'y); auto.
+  - destruct H as [y' [x'y' y't]].
+    rewrite <- Ex' in x'y'.
+    commute x x' y' xx' x'y' as y; exists y.
+    split; [rewrite <- Ex; auto|].
+    transitivity y'; auto.
+    rewrite yy'; auto.
+Qed.
+
+Instance conv_proper_pi (Var : Set) : Proper (pi --> impl) (@conv Var).
+Proof.
+  intros x x' xx' [y [xy yt]];
+  wlog_closed x; wlog_closed x';
+  apply pi_close in xx'; rewrite <- Ex in xx'; rewrite <- Ex' in xx'.
+  rewrite <- Ex in xy.
+  commute x' x y xx' xy as y'; exists y'.
+  split; [rewrite <- Ex'; auto| eauto].
+Qed.
+
+Instance conv_proper_probe (Var : Set) : Proper (probe ==> iff) (@conv Var).
+Proof.
+  intros x x' xx'; split; intro H;
+  wlog_closed x; wlog_closed x';
+  apply probe_close in xx'; rewrite <- Ex in xx'; rewrite <- Ex' in xx'.
+  - destruct H as [y [xy yt]].
+    rewrite <- Ex in xy.
+    commute x' x y xx' xy as y'; exists y'.
+    split; [rewrite <- Ex'; auto|].
+    apply probe_pi_top with y; auto.
+  - destruct H as [y' [x'y' y't]].
+    exists y'; split; auto.
+    rewrite <- Ex' in x'y'.
+    transitivity x'; auto.
+    rewrite <- Ex; auto.
+Qed.
+
+Lemma conv_top (Var : Set) : conv (TOP : Term Var).
+Proof.
+  exists TOP; split; auto.
+Qed.
+Hint Resolve conv_top.
+
+(** ** A [heads] relation for proving nontermination *)
+
+Inductive heads {Var : Set} : relation (Term Var) :=
+  | heads_refl x : heads x x
+  | heads_ap h x y : heads h x -> heads h (x * y).
+
+Ltac heads :=
+  auto using heads_refl, heads_ap;
+  match goal with
+  | [H : heads ?x ?y |- _] => inversion_clear H; heads
+  end.
+
+Lemma heads_close (Var : Set) (h x : Term Var) :
+  heads h x -> heads (close h) (close x).
+Proof.
+  intro H; induction H; simpl; compute; heads.
+Qed.
+
+Lemma heads_probe (Var : Set) (h x y : Term Var) :
+  probe x y -> heads h x -> heads h y.
+Proof.
+  rewrite weaken_probe.
+  intro xy; induction xy; simpl_probe_step; heads.
+Qed.
+
+Lemma heads_beta_bot (Var : Set) (x y : Term Var) :
+  beta x y -> heads BOT x -> heads BOT y.
+Proof.
+  intros Ht; induction Ht; intros; heads.
+Qed.
+
+Lemma heads_pi_bot (Var : Set) (x y : Term Var) :
+  pi x y -> heads BOT x -> heads BOT y.
+Proof.
+  intros Ht; induction Ht; intros; heads.
+Qed.
+
+Lemma not_conv_heads_bot (Var : Set) (x : Term Var) : heads BOT x -> ~ conv x.
+Proof.
+  intros H [y [xy yt]].
+  apply (heads_close) in H.
+  apply (heads_probe _ _ _ y) in H; auto.
+  apply (heads_pi_bot _ _ TOP) in H; auto.
+  inversion H; auto.
+Qed.
+
+Lemma not_conv_bot (Var : Set) : ~ conv (BOT : Term Var).
+Proof.
+  apply not_conv_heads_bot; heads.
+Qed.
+Hint Resolve not_conv_bot.
