src/Reduction.v
@@ -1,0 +1,622 @@
+(** * Reduction relations *)
+
+Require Import Coq.Program.Basics.
+Require Import Coq.Program.Equality.
+Require Import Coq.Setoids.Setoid.
+Require Import Coq.Classes.RelationClasses.
+Require Import Coq.Classes.Morphisms.
+Require Export Substitution.
+
+Inductive star {Var : Set} (r : relation (Term Var)) : relation (Term Var) :=
+  | star_step {x y} : r x y -> star r x y
+  | star_refl {x} : star r x x
+  | star_trans {x} y {z} : star r x y -> star r y z -> star r x z.
+Hint Constructors star.
+
+Inductive weak_star
+  {Var : Set} (r : relation (Term Var)) : relation (Term Var) :=
+  | weak_star_refl {x} : weak_star r x x
+  | weak_star_trans {x} y {z} : r x y -> weak_star r y z -> weak_star r x z.
+Hint Constructors weak_star.
+
+Lemma weaken_star (Var : Set) (r : relation (Term Var)) (x y : Term Var) :
+  star r x y <-> weak_star r x y.
+Proof.
+  split; intro H; induction H; eauto.
+  clear H H0; induction IHstar1; auto.
+  apply weak_star_trans with y; auto.
+Qed.
+
+Lemma weak_star_flip (Var : Set) (r : relation (Term Var)) (x y : Term Var) :
+  weak_star (flip r) x y <-> weak_star r y x.
+Proof.
+  repeat rewrite <- weaken_star.
+  split; intro H; induction H; eauto.
+Qed.
+
+
+Inductive probe {Var : Set} : relation (Term Var) :=
+  | probe_refl {x} : probe x x
+  | probe_trans {x} y {z} : probe x y -> probe y z -> probe x z
+  | probe_top {x} : probe x (x * TOP).
+Hint Constructors probe.
+
+Inductive probe_step {Var : Set} : relation (Term Var) :=
+  | probe_step_top {x} : probe_step x (x * TOP).
+Hint Constructors probe_step.
+
+Lemma weaken_probe (Var : Set) (x y : Term Var) :
+  probe x y <-> weak_star probe_step x y.
+Proof.
+  rewrite <- weaken_star.
+  split; intro H; induction H; eauto.
+  inversion H; auto.
+Qed.
+
+Definition lambda_app_sub {Var : Set} (x : Term (option Var)) (y : Term Var) :
+  Term Var := x @ (fun v => match v with None => y | Some v' => VAR v' end).
+
+Inductive beta {Var : Set} : relation (Term Var) :=
+  | beta_refl {x} : beta x x
+  | beta_trans {x} y {z} : beta x y -> beta y z -> beta x z
+  | beta_app_left {x x' y} : beta x x' -> beta (x * y) (x' * y)
+  | beta_app_right {x y y'} : beta y y' -> beta (x * y) (x * y')
+  | beta_join_left {x x' y} : beta x x' -> beta (x || y) (x' || y)
+  | beta_join_right {x y y'} : beta y y' -> beta (x || y) (x || y')
+  | beta_rand_left {x x' y} : beta x x' -> beta (x (+) y) (x' (+) y)
+  | beta_rand_right {x y y'} : beta y y' -> beta (x (+) y) (x (+) y')
+  | beta_lambda {x x'} :
+      @beta (option Var) x x' -> beta (LAMBDA x) (LAMBDA x')
+  | beta_sub {x y} : beta (LAMBDA x * y) (lambda_app_sub x y)
+  | beta_j_ap {x y z} : beta ((x || y) * z) (x * z || y * z)
+  | beta_r_ap {x y z} : beta ((x (+) y) * z) (x * z (+) y * z)
+  | beta_r_idem {x} : beta (x (+) x) x
+  | beta_r_sym {x y} : beta (x (+) y) (y (+) x)
+  | beta_r_sym_sym {w x y z} :
+      beta ((w(+)x) (+) (y(+)z)) ((x(+)y) (+) (z(+)w)).
+Hint Constructors beta.
+
+Inductive beta_step {Var : Set} : relation (Term Var) :=
+  | beta_step_app_left {x x' y} : beta_step x x' -> beta_step (x * y) (x' * y)
+  | beta_step_app_right {x y y'} : beta_step y y' -> beta_step (x * y) (x * y')
+  | beta_step_join_left {x x' y} :
+      beta_step x x' -> beta_step (x || y) (x' || y)
+  | beta_step_join_right {x y y'} :
+      beta_step y y' -> beta_step (x || y) (x || y')
+  | beta_step_rand_left {x x' y} :
+      beta_step x x' -> beta_step (x (+) y) (x' (+) y)
+  | beta_step_rand_right {x y y'} :
+      beta_step y y' -> beta_step (x (+) y) (x (+) y')
+  | beta_step_lambda {x x'} :
+      @beta_step (option Var) x x' -> beta_step (LAMBDA x) (LAMBDA x')
+  | beta_step_sub {x y} : beta_step (LAMBDA x * y) (lambda_app_sub x y)
+  | beta_step_j_ap {x y z} : beta_step ((x || y) * z) (x * z || y * z)
+  | beta_step_r_ap {x y z} : beta_step ((x (+) y) * z) (x * z (+) y * z)
+  | beta_step_r_idem {x} : beta_step (x (+) x) x
+  | beta_step_r_sym {x y} : beta_step (x (+) y) (y (+) x)
+  | beta_step_r_sym_sym {w x y z} :
+      beta_step ((w(+)x) (+) (y(+)z)) ((x(+)y) (+) (z(+)w)).
+Hint Constructors beta_step.
+
+Lemma weaken_beta (Var : Set) (x y : Term Var) :
+  beta x y <-> weak_star beta_step x y.
+Proof.
+  rewrite <- weaken_star.
+  split; intro H; induction H; eauto;
+  match goal with
+  | [IH : star _ _ _ |- star _ _ _ ] => clear H; induction IH; eauto
+  | _ => induction H; auto
+  end.
+Qed.
+
+
+Inductive pi {Var : Set} : relation (Term Var) :=
+  | pi_refl {x} : pi x x
+  | pi_trans {x} y {z} : pi x y -> pi y z -> pi x z
+  | pi_app_left {x x' y} : pi x x' -> pi (x * y) (x' * y)
+  | pi_app_right {x y y'} : pi y y' -> pi (x * y) (x * y')
+  | pi_join_left {x x' y} : pi x x' -> pi (x || y) (x' || y)
+  | pi_join_right {x y y'} : pi y y' -> pi (x || y) (x || y')
+  | pi_rand_left {x x' y} : pi x x' -> pi (x (+) y) (x' (+) y)
+  | pi_rand_right {x y y'} : pi y y' -> pi (x (+) y) (x (+) y')
+  | pi_lambda {x x'} : @pi (option Var) x x' -> pi (LAMBDA x) (LAMBDA x')
+  | pi_sub {x y} : pi (LAMBDA x * y) (lambda_app_sub x y)
+  | pi_j_ap {x y z} : pi ((x || y) * z) (x * z || y * z)
+  | pi_r_ap {x y z} : pi ((x (+) y) * z) (x * z (+) y * z)
+  | pi_r_idem {x} : pi (x (+) x) x
+  | pi_r_sym {x y} : pi (x (+) y) (y (+) x)
+  | pi_r_sym_sym {w x y z} :
+      pi ((w(+)x) (+) (y(+)z)) ((x(+)y) (+) (z(+)w))
+  | pi_top x : pi TOP x
+  | pi_bot x : pi x BOT
+  | pi_j_left {x y} : pi (x || y) x
+  | pi_j_right {x y} : pi (x || y) y.
+Hint Constructors pi.
+
+Inductive pi_step {Var : Set} : relation (Term Var) :=
+  | pi_step_app_left {x x' y} : pi_step x x' -> pi_step (x * y) (x' * y)
+  | pi_step_app_right {x y y'} : pi_step y y' -> pi_step (x * y) (x * y')
+  | pi_step_join_left {x x' y} : pi_step x x' -> pi_step (x || y) (x' || y)
+  | pi_step_join_right {x y y'} : pi_step y y' -> pi_step (x || y) (x || y')
+  | pi_step_rand_left {x x' y} : pi_step x x' -> pi_step (x (+) y) (x' (+) y)
+  | pi_step_rand_right {x y y'} : pi_step y y' -> pi_step (x (+) y) (x (+) y')
+  | pi_step_lambda {x x'} :
+      @pi_step (option Var) x x' -> pi_step (LAMBDA x) (LAMBDA x')
+  | pi_step_sub {x y} : pi_step (LAMBDA x * y) (lambda_app_sub x y)
+  | pi_step_j_ap {x y z} : pi_step ((x || y) * z) (x * z || y * z)
+  | pi_step_r_ap {x y z} : pi_step ((x (+) y) * z) (x * z (+) y * z)
+  | pi_step_r_idem {x} : pi_step (x (+) x) x
+  | pi_step_r_sym {x y} : pi_step (x (+) y) (y (+) x)
+  | pi_step_r_sym_sym {w x y z} :
+      pi_step ((w(+)x) (+) (y(+)z)) ((x(+)y) (+) (z(+)w))
+  | pi_step_top x : pi_step TOP x
+  | pi_step_bot x : pi_step x BOT
+  | pi_step_j_left {x y} : pi_step (x || y) x
+  | pi_step_j_right {x y} : pi_step (x || y) y.
+Hint Constructors pi_step.
+
+Lemma weaken_pi (Var : Set) (x y : Term Var) :
+  pi x y <-> weak_star pi_step x y.
+Proof.
+  rewrite <- weaken_star.
+  split; intro H; induction H; eauto;
+  match goal with
+  | [IH : star _ _ _ |- star _ _ _ ] => clear H; induction IH; eauto
+  | _ => induction H; auto
+  end.
+Qed.
+
+
+Hint Rewrite @beta_j_ap @beta_r_ap @beta_r_idem : beta_safe.
+Hint Rewrite @beta_sub : beta_unsafe.
+
+Tactic Notation "beta_simpl" :=
+  autorewrite with term_simpl beta_safe.
+Tactic Notation "beta_simpl" "in" hyp(H) :=
+  autorewrite with term_simpl beta_safe in H.
+Tactic Notation "beta_reduce" :=
+  autorewrite with term_simpl beta_safe beta_unsafe.
+Tactic Notation "beta_reduce" "in" hyp(H) :=
+  autorewrite with term_simpl beta_safe beta_unsafe in H.
+
+(** To avoid nontermination in [beta_reduce],
+    we provide a mechanism to "freeze" terms during reduction. *)
+Tactic Notation "freeze" reference(c) "in" tactic(tac) :=
+  let v := fresh "v" in
+  let H := fresh "Hv" in
+  assert (exists v, c=v) as H;
+  [ exists c; reflexivity
+  | destruct H as [v H]; rewrite H; tac; destruct H].
+
+
+Class Commuting (Var : Set) (r s : relation (Term Var)) :=
+  commuting : forall x y z, r x y -> s y z -> exists y', s x y' /\ r y' z.
+
+Tactic Notation
+  "commute" ident(x) ident(y) ident(z) constr(xy) constr(yz)
+  "as" ident(w) :=
+  let xy := fresh x y in
+  let yx := fresh y x in
+  let yz := fresh y z in
+  let zy := fresh z y in
+  let xw := fresh x w in
+  let wz := fresh w z in
+  let H := fresh in
+  match type of xy with
+    | ?r y x => assert (flip r x y) as xy; [unfold flip; assumption | idtac]
+    | ?r x y => idtac
+  end;
+  match type of yz with
+    | ?r z y => assert (flip r y z) as yz; [unfold flip; assumption | idtac]
+    | ?r y z => idtac
+  end;
+  set (H := commuting x y z xy yz);
+  destruct H as [w [xw wz]];
+  try unfold flip in xw, wz.
+
+Lemma weaken_commuting (Var : Set) (r s r' s' : relation (Term Var)) :
+  (forall (x y : Term Var), r x y <-> weak_star r' x y) ->
+  (forall (x y : Term Var), s x y <-> weak_star s' x y) ->
+  (forall x y z, r' x y -> s' y z -> exists y', s x y' /\ r y' z) ->
+  Commuting Var r s.
+Proof.
+  intros Hr Hs Hweak x y z rxy syz.
+  rewrite Hr in rxy.
+  rewrite Hs in syz.
+  induction rxy; induction syz; eauto.
+  - exists x; rewrite Hr, Hs; auto.
+  - exists z; rewrite Hr, Hs; split; auto.
+    apply weak_star_trans with y; auto.
+  - exists x; rewrite Hr, Hs; split; auto.
+    apply weak_star_trans with y; auto.
+  - admit. (* TODO also assume r == star r and s == star s,
+              then use strong induction *)
+Qed.
+
+
+Instance probe_reflexive (Var : Set) : Reflexive (@probe Var).
+Proof.
+  auto.
+Qed.
+
+Instance probe_transitive (Var : Set) : Transitive (@probe Var).
+Proof.
+  intros x y z; apply probe_trans.
+Qed.
+
+Instance probe_preorder (Var : Set) : PreOrder (@probe Var).
+Proof.
+  split; [apply probe_reflexive | apply probe_transitive].
+Qed.
+
+Lemma probe_step_probe (Var : Set) (x y : Term Var) :
+  probe_step x y -> probe x y.
+Proof.
+  intro H; inversion H; auto.
+Qed.
+
+Ltac simpl_probe_step :=
+  repeat
+  match goal with
+    | [H : probe_step _ _ |- _] => destruct H
+  (*
+    | [|- probe ?x ?y] => rewrite weaken_probe
+    | [H : star probe_step _ _ |- _] => induction H
+  *)
+    | [H : probe_step ?x ?x -> _ |- _] => clear H
+  end;
+  eauto.
+
+Instance commuting_flip_probe_probe (Var : Set) :
+  Commuting Var (flip probe) probe.
+Proof.
+  apply (weaken_commuting _ _ _ (flip probe_step) probe_step); auto.
+  - intros x y; rewrite weak_star_flip; compute; apply weaken_probe.
+  - apply weaken_probe.
+  - unfold flip; intros x y z xy yz.
+    induction xy; induction yz; eauto.
+Qed.
+
+
+Instance beta_reflexive (Var : Set) : Reflexive (@beta Var).
+Proof.
+  auto.
+Qed.
+
+Instance beta_transitive (Var : Set) : Transitive (@beta Var).
+Proof.
+  intros x y z; apply beta_trans.
+Qed.
+
+Instance beta_preorder (Var : Set) : PreOrder (@beta Var).
+Proof.
+  split; [apply beta_reflexive | apply beta_transitive].
+Qed.
+
+Instance beta_step_subrelation (Var : Set) :
+  (@subrelation (Term Var)) beta_step beta.
+Proof.
+  intros x y H; induction H; eauto.
+Qed.
+
+Instance APP_beta (Var : Set) :
+  Proper (beta ==> beta ==> beta) (@APP Var).
+Proof.
+  intros x x' Hx y y' Hy; transitivity (x * y'); auto.
+Qed.
+
+Ltac simpl_beta_step :=
+  (* repeat *)
+  match goal with
+    | [H : beta_step _ _ |- _] => induction H
+    | [H : beta_step ?x ?x -> _ |- _] => clear H
+  end.
+
+Lemma beta_step_beta (Var : Set) (x y : Term Var) :
+  beta_step x y -> beta x y.
+Proof.
+  intro H; induction H; auto.
+Qed.
+
+Instance commuting_flip_beta_beta (Var : Set) : Commuting Var (flip beta) beta.
+Proof.
+  apply (weaken_commuting _ _ _ (flip beta_step) beta_step); auto.
+  - intros x y; rewrite weak_star_flip; compute; apply weaken_beta.
+  - apply weaken_beta.
+  - compute; intros x y z xy yz.
+    (* TODO try induction over just one variable,
+       mapping beta to beta.
+       The only problem is with steps that are the same (use refl)
+       and in beta_r_ when redexes intersect.
+       Try to write a tactic matching against beta constructors. *)
+    (* OLD
+    induction xy; induction yz; auto.
+    *)
+Admitted. 
+
+Instance commuting_flip_beta_probe (Var : Set) :
+  Commuting Var (flip beta) probe.
+Proof.
+  apply (weaken_commuting _ _ _ (flip beta_step) probe_step); auto.
+  - intros x y; rewrite weak_star_flip; compute; apply weaken_beta.
+  - apply weaken_probe.
+  - compute; intros x y z xy yz.
+    destruct yz.
+    exists (x * TOP); repeat split; auto.
+    apply (@weak_star_trans _ _ x0 x x) in xy; auto.
+    rewrite <- weaken_beta in xy; auto.
+Qed.
+
+Instance commuting_beta_probe (Var : Set) : Commuting Var beta probe.
+Proof.
+  apply (weaken_commuting _ _ _ beta_step probe_step); auto.
+  - apply weaken_beta.
+  - apply weaken_probe.
+  - compute; intros x y z xy yz; destruct yz; exists (x * TOP); split; auto.
+    rewrite xy; reflexivity.
+Qed.
+
+
+Instance pi_reflexive (Var : Set) : Reflexive (@pi Var).
+Proof.
+  auto.
+Qed.
+
+Instance pi_transitive (Var : Set) : Transitive (@pi Var).
+Proof.
+  intros x y z; apply pi_trans.
+Qed.
+
+Instance pi_preorder (Var : Set) : PreOrder (@pi Var).
+Proof.
+  split; [apply pi_reflexive | apply pi_transitive].
+Qed.
+
+Instance pi_step_pi_subrelation (Var : Set) :
+  (@subrelation (Term Var)) pi_step pi.
+Proof.
+  intros x y H; induction H; eauto.
+Qed.
+
+Instance beta_step_pi_subrelation (Var : Set) :
+  (@subrelation (Term Var)) beta_step pi.
+Proof.
+  intros x y H; induction H; eauto.
+Qed.
+
+Instance beta_pi_subrelation (Var : Set) : (@subrelation (Term Var)) beta pi.
+Proof.
+  intros x y Hb; induction Hb; eauto.
+Qed.
+
+Instance pi_proper_beta (Var : Set) : Proper (beta --> beta ++> impl) (@pi Var).
+Proof.
+  intros x x' xx' y y' yy' Hp; compute in yy'.
+  apply beta_pi_subrelation in xx'; rewrite xx'.
+  apply beta_pi_subrelation in yy'; rewrite <- yy'.
+  auto.
+Qed.
+
+Instance APP_pi (Var : Set) :
+  Proper (pi ==> pi ==> pi) (@APP Var).
+Proof.
+  intros x x' Hx y y' Hy; transitivity (x * y'); auto.
+Qed.
+
+Ltac simpl_pi_step :=
+  (* repeat *)
+  match goal with
+    | [H : pi_step _ _ |- _] => induction H
+    | [H : pi_step ?x ?x -> _ |- _] => clear H
+  end.
+
+Lemma pi_step_pi (Var : Set) (x y : Term Var) :
+  pi_step x y -> pi x y.
+Proof.
+  intro H; induction H; auto.
+Qed.
+
+Instance commuting_flip_pi_pi (Var : Set) : Commuting Var (flip pi) pi.
+Proof.
+  apply (weaken_commuting _ _ _ (flip pi_step) pi_step); auto.
+  - intros x y; rewrite weak_star_flip; compute; apply weaken_pi.
+  - apply weaken_pi.
+  - compute; intros x y z xy yz.
+    (* TODO similar to commuting_flip_beta_beta *)
+    (* OLD
+    induction xy; induction yz; auto.
+    *)
+Admitted. 
+
+Instance commuting_flip_pi_probe (Var : Set) :
+  Commuting Var (flip pi) probe.
+Proof.
+  apply (weaken_commuting _ _ _ (flip pi_step) probe_step); auto.
+  - intros x y; rewrite weak_star_flip; compute; apply weaken_pi.
+  - apply weaken_probe.
+  - compute; intros x y z xy yz.
+    destruct yz.
+    exists (x * TOP); repeat split; auto.
+    apply (@weak_star_trans _ _ x0 x x) in xy; auto.
+    rewrite <- weaken_pi in xy; auto.
+Qed.
+
+Instance commuting_pi_probe (Var : Set) : Commuting Var pi probe.
+Proof.
+  apply (weaken_commuting _ _ _ pi_step probe_step); auto.
+  - apply weaken_pi.
+  - apply weaken_probe.
+  - compute; intros x y z xy yz; destruct yz; exists (x * TOP); split; auto.
+    rewrite xy; reflexivity.
+Qed.
+
+(* TODO try to replace this with commuting_beta_step_pi
+   since [beta TOP x -> x == TOP]? *)
+Lemma beta_step_pi_top (Var : Set) (x y : Term Var) :
+  beta_step x y -> (pi x TOP <-> pi y TOP).
+Proof.
+  intro Hb; split; intro Hp.
+  - admit. (* TODO similar strategy to commuting_flip_beta_beta *)
+  - rewrite Hb; auto.
+Qed.
+
+Lemma beta_pi_top (Var : Set) (x y : Term Var) :
+  beta x y -> (pi x TOP <-> pi y TOP).
+Proof.
+  intro Hb; rewrite weaken_beta in Hb; induction Hb; try tauto.
+  transitivity (pi y TOP); auto.
+  apply beta_step_pi_top; auto.
+Qed.
+
+Lemma probe_pi_top (Var : Set) (x y : Term Var) :
+  probe x y -> pi x TOP -> pi y TOP.
+Proof.
+  intro Hp; rewrite weaken_probe in Hp; induction Hp; try tauto.
+  destruct H; intro H; apply IHHp.
+  transitivity (TOP * TOP : Term Var); auto.
+  transitivity (K * TOP * TOP : Term Var); auto.
+  unfold K.
+  rewrite beta_sub; compute.
+  rewrite beta_sub; compute.
+  auto.
+Qed.
+
+
+
+Lemma term_sub_proper_probe (Var Var' : Set)
+  (f : Var -> Term Var') (x y : Term Var) :
+  probe x y -> probe (x @ f) (y @ f).
+Proof.
+  intro xy; induction xy; simpl.
+  - reflexivity.
+  - transitivity (y @ f); auto.
+  - apply probe_top; auto.
+Qed.
+
+Lemma term_sub_beta_left
+  (Var Var' : Set) (f g : Var -> Term Var') (x : Term Var) :
+  (forall v, beta (f v) (g v)) -> beta (x @ f) (x @ g).
+Proof.
+  intros fg; induction x; auto.
+  - simpl; transitivity ((x1 @ g) || (x2 @ f)); auto.
+  - simpl; transitivity ((x1 @ g) (+) (x2 @ f)); auto.
+  - simpl; transitivity ((x1 @ g) * (x2 @ f)); auto.
+  - simpl; auto.
+  - apply beta_lambda.
+    admit.
+    (* TODO how to do heterogeneous induction? *)
+Qed.
+Hint Resolve term_sub_beta_left.
+
+Lemma term_sub_beta_right
+  (Var Var' : Set) (f : Var -> Term Var') (x y : Term Var) :
+  beta x y -> beta (x @ f) (y @ f).
+Proof.
+  intro xy; induction xy; repeat rewrite term_sub_ap;
+  try (simpl; auto; reflexivity).
+  - transitivity (y @ f); auto.
+  - admit.
+  - admit.
+Qed.
+Hint Resolve term_sub_beta_right.
+
+Instance term_sub_proper_beta (Var Var' : Set) :
+  Proper ((eq ==> beta) ==> beta ==> beta) (@term_sub Var Var').
+Proof.
+  intros f g Hfg x y Hxy; transitivity (y @ f);
+  [apply term_sub_beta_right | apply term_sub_beta_left]; auto.
+Qed.
+
+Lemma term_sub_pi_left
+  (Var Var' : Set) (f g : Var -> Term Var') (x : Term Var) :
+  (forall v, pi (f v) (g v)) -> pi (x @ f) (x @ g).
+Proof.
+  intros fg; induction x; auto.
+  - simpl; transitivity ((x1 @ f) || (x2 @ g)); auto.
+  - simpl; transitivity ((x1 @ f) (+) (x2 @ g)); auto.
+  - simpl; transitivity ((x1 @ f) * (x2 @ g)); auto.
+  - admit.
+  - admit.
+Qed.
+Hint Resolve term_sub_pi_left.
+
+Lemma term_sub_pi_right
+  (Var Var' : Set) (f : Var -> Term Var') (x y : Term Var) :
+  pi x y -> pi (x @ f) (y @ f).
+Proof.
+  intro xy; induction xy; repeat rewrite term_sub_ap; simpl; auto.
+  - transitivity (y @ f); auto.
+  - admit.
+  - admit.
+Qed.
+Hint Resolve term_sub_pi_right.
+
+Instance term_sub_proper_pi (Var Var' : Set) :
+  Proper ((eq ==> pi) ==> pi ==> pi) (@term_sub Var Var').
+Proof.
+  intros f g Hfg x y Hxy; transitivity (y @ f);
+  [apply term_sub_pi_right | apply term_sub_pi_left]; auto.
+Qed.
+
+Instance term_close_proper_beta (Var : Set) :
+  Proper (beta ==> beta) (@close Var).
+Proof.
+  intros x x' xx'; apply weaken_beta in xx'; induction xx'; auto.
+  revert z xx' IHxx'; induction H; intros;
+  try (compute; term_simpl; eauto; reflexivity).
+  - admit.
+  - admit.
+Qed.
+
+Instance term_close_proper_pi (Var : Set) :
+  Proper (pi ==> pi) (@close Var).
+Proof.
+  intros x x' xx'; apply weaken_pi in xx'; induction xx'; auto.
+  revert z xx' IHxx'; induction H; intros;
+  try (compute; term_simpl; eauto; reflexivity).
+  - admit.
+  - admit.
+Qed.
+
+Lemma probe_step_close (Var : Set) (x y : Term Var) :
+  probe_step x y -> probe (close x) (close y).
+Proof.
+  intro Hb; induction Hb; compute; auto.
+Qed.
+
+Lemma probe_close (Var : Set) (x y : Term Var) :
+  probe x y -> probe (close x) (close y).
+Proof.
+  intro Hb; rewrite weaken_probe in Hb; induction Hb; auto.
+  rewrite <- IHHb; clear Hb IHHb; auto using probe_step_close.
+Qed.
+
+Lemma beta_step_close (Var : Set) (x y : Term Var) :
+  beta_step x y -> beta (close x) (close y).
+Proof.
+  intro Hb; induction Hb; try (compute; beta_reduce; auto).
+  - admit.
+  - admit.
+Qed.
+
+Lemma beta_close (Var : Set) (x y : Term Var) :
+  beta x y -> beta (close x) (close y).
+Proof.
+  intro Hb; rewrite weaken_beta in Hb; induction Hb; auto.
+  rewrite <- IHHb; clear Hb IHHb; auto using beta_step_close.
+Qed.
+
+Lemma pi_step_close (Var : Set) (x y : Term Var) :
+  pi_step x y -> pi (close x) (close y).
+Proof.
+  intro Hb; induction Hb; try (compute; beta_reduce; auto).
+  - admit.
+  - admit.
+Qed.
+
+Lemma pi_close (Var : Set) (x y : Term Var) :
+  pi x y -> pi (close x) (close y).
+Proof.
+  intro Hb; rewrite weaken_pi in Hb; induction Hb; auto.
+  rewrite <- IHHb; clear Hb IHHb; auto using pi_step_close.
+Qed.
