src/Substitution.v
@@ -1,0 +1,155 @@
+(** * Substitution *)
+
+Require Import Coq.Program.Equality.
+Require Import Coq.Setoids.Setoid.
+Require Import Coq.Classes.Morphisms.
+Require Export Terms.
+
+(* adapted from https://coq.inria.fr/cocorico/UntypedLambdaTerms *)
+
+Fixpoint term_map {Var Var' : Set} (f : Var -> Var') (x : Term Var) :
+  Term Var' :=
+  match x with
+  | TOP => TOP
+  | BOT => BOT
+  | x1 || x2 => term_map f x1 || term_map f x2
+  | x1 (+) x2 => term_map f x1 (+) term_map f x2
+  | x1 * x2 => term_map f x1 * term_map f x2
+  | VAR x => VAR (f x)
+  | LAMBDA x1 => LAMBDA (term_map (option_map f) x1)
+  end.
+
+Fixpoint term_sub {Var Var' : Set} (f : Var -> Term Var') (x : Term Var) :
+  Term Var' :=
+  match x with
+  | TOP => TOP
+  | BOT => BOT
+  | x1 || x2 => term_sub f x1 || term_sub f x2
+  | x1 (+) x2 => term_sub f x1 (+) term_sub f x2
+  | x1 * x2 => term_sub f x1 * term_sub f x2
+  | VAR v => f v
+  | LAMBDA x1 => LAMBDA (term_sub (fun x => 
+    match x with
+    | None => VAR None
+    | Some y => term_map (@Some Var') (f y)
+    end) x1)
+  end.
+
+Instance term_sub_proper (Var Var' : Set) :
+  Proper ((eq ==> eq) ==> eq ==> eq) (@term_sub Var Var').
+Proof.
+  intros f f' ff'; compute in ff'.
+  intros x x' xx'; rewrite <- xx'; clear x' xx'.
+  induction x; auto.
+  - simpl; rewrite (IHx1 f f'), (IHx2 f f'); auto.
+  - simpl; rewrite (IHx1 f f'), (IHx2 f f'); auto.
+  - simpl; rewrite (IHx1 f f'), (IHx2 f f'); auto.
+  - compute; auto.
+  - admit.
+    (* TODO how to do heterogeneous induction? *)
+Qed.
+
+Notation "x @ f" := (term_sub f x) : term_scope.
+
+Definition sub_top {Var : Set} (v : Var) : Closed := TOP.
+Definition close {Var : Set} : Term Var -> Closed := term_sub sub_top.
+
+Tactic Notation "term_simpl" := autorewrite with term_simpl.
+Tactic Notation "term_simpl" "in" hyp(H) := autorewrite with term_simpl in H.
+
+Lemma var_monad_unit_right (Var : Set) (x : Term Var) : x @ VAR = x.
+Proof.
+  induction x; auto; simpl;
+  repeat
+    match goal with
+    | [H : _ @ VAR = _ |- _] => rewrite H; clear H
+    end;
+  try reflexivity.
+  admit.
+Qed.
+Hint Rewrite var_monad_unit_right : term_simpl.
+
+Lemma var_monad_unit_left (Var Var' : Set) (f : Var -> Term Var') x :
+  (VAR x) @ f = f x.
+Proof.
+  compute; auto.
+Qed.
+Hint Rewrite var_monad_unit_left : term_simpl.
+
+Lemma term_sub_ap (Var Var' : Set) (x y : Term Var) (f : Var -> Term Var') :
+  (x * y @ f) = (x @ f) * (y @ f).
+Proof.
+  simpl; auto.
+Qed.
+Hint Rewrite term_sub_ap : term_simpl.
+
+Lemma term_sub_join (Var Var' : Set) (x y : Term Var) (f : Var -> Term Var') :
+  (x || y @ f) = (x @ f) || (y @ f).
+Proof.
+  simpl; auto.
+Qed.
+Hint Rewrite term_sub_join : term_simpl.
+
+Lemma term_sub_rand (Var Var' : Set) (x y : Term Var) (f : Var -> Term Var') :
+  (x (+) y @ f) = (x @ f) (+) (y @ f).
+Proof.
+  simpl; auto.
+Qed.
+Hint Rewrite term_sub_rand : term_simpl.
+
+Definition lambda_map
+  {Var Var' : Set} (f : Var -> Term Var') (v : option Var) :
+  Term (option Var') :=
+  match v with
+  | None => VAR None
+  | Some v' => term_map (@Some Var') (f v')
+  end.
+
+Lemma term_sub_lambda
+  (Var Var' : Set) (x : Term (option Var)) (f : Var -> Term Var') :
+  (LAMBDA x @ f) = LAMBDA (x @ lambda_map f).
+Proof.
+  simpl; auto.
+Qed.
+Hint Rewrite term_sub_lambda : term_simpl.
+
+Lemma var_monad_assoc
+  (Var Var' Var'' : Set)
+  (f : Var -> Term Var')
+  (g : Var' -> Term Var'')
+  (x : Term Var) :
+  (x @ f) @ g = x @ (fun v => (f v) @ g).
+Proof.
+  induction x; auto.
+  - term_simpl; rewrite IHx1; rewrite IHx2; auto.
+  - term_simpl; rewrite IHx1; rewrite IHx2; auto.
+  - term_simpl; rewrite IHx1; rewrite IHx2; auto.
+  - term_simpl. (* rewrite IHx; auto. *)
+    admit.
+    (* TODO how to do heterogeneous induction? *)
+Qed.
+Hint Rewrite var_monad_assoc : term_simpl.
+
+Lemma close_idempotent (Var : Set) (x : Term Var) : close (close x) = close x.
+Proof.
+  compute; term_simpl; induction x; auto.
+Qed.
+Hint Rewrite close_idempotent : beta_simpl.
+Hint Rewrite close_idempotent : term_simpl.
+
+Lemma close_closed (x : Closed) : close x = x.
+Proof.
+  unfold Closed in x; unfold close, sub_top.
+  dependent induction x; term_simpl;
+  match goal with [v : Empty_set |- _] => destruct v | _ => idtac end; auto.
+  - rewrite IHx1; rewrite IHx2; reflexivity.
+  - rewrite IHx1; rewrite IHx2; reflexivity.
+  - rewrite IHx1; rewrite IHx2; reflexivity.
+  - clear IHx.
+    set (f := lambda_map (fun _ : Empty_set => TOP)).
+    assert (x @ f = x) as Eq1; [| rewrite Eq1; reflexivity].
+    admit.
+    (* TODO prove a stronger lemma that implies this lemma *)
+Qed.
+Hint Rewrite close_closed : beta_simpl.
+Hint Rewrite close_closed : term_simpl.
