src/make.sh
@@ -1,8 +1,4 @@
 #!/bin/sh
 
-# Coq 8.4+ 
-coq_makefile -install none *.v > Makefile
-# Coq <8.4
-#coq_makefile -no-install *.v > Makefile
-
+coq_makefile *.v -install none -o Makefile
 make
